soundness/FallingEdge.v
@@ -1,0 +1,49 @@
+(** * Falling Edge Lemma *)
+
+Require Import common.NatMap.
+
+Require Import sitpn.dp.SitpnTypes.
+Require Import sitpn.dp.SitpnSemantics.
+
+Require Import hvhdl.AbstractSyntax.
+Require Import hvhdl.SemanticalDomains.
+Require Import hvhdl.Stabilize.
+Require Import hvhdl.SynchronousEvaluation.
+Require Import hvhdl.Environment.
+Require Import hvhdl.DesignElaboration.
+Require Import hvhdl.HilecopDesignStore.
+
+Require Import sitpn2hvhdl.GenerateHVhdl.
+
+Require Import soundness.SoundnessDefs.
+
+(** ** Falling Edge Lemma *)
+
+Lemma falling_edge :
+  forall sitpn decpr id__ent id__arch mm d γ E__c E__p Δ σ__e s σ τ s' σ__injf σ__f σ' θ,
+
+    (* sitpn translates into (d, γ). *)
+    sitpn_to_hvhdl sitpn decpr id__ent id__arch mm = (inl (d, γ)) ->
+
+    (* Environments are similar. *)
+    SimEnv sitpn γ E__c E__p ->
+    
+    (* [Δ, σ__e] are the results of the elaboration of [d]. *)
+    edesign hdstore (empty value) d Δ σ__e ->
+
+    (* States s and σ are similar (post rising edge). *)
+    SimStateAfterRE sitpn γ s σ ->
+
+    (* From s to s' after ↓. *)
+    SitpnStateTransition E__c τ s s' fe ->
+
+    (* From σ to σ' after ↓. *)
+    IsInjectedDState σ (E__p τ fe) σ__injf ->
+    vfalling Δ σ__injf (behavior d) σ__f ->
+    stabilize Δ σ__f (behavior d) θ σ' ->
+
+    (* States s' and σ' are similar (post falling edge). *)
+    SimStateAfterFE sitpn γ s' σ'.
+Admitted.
+
+Hint Resolve falling_edge : core.
