soundness/FallingEdgeFacts.v
@@ -41,7 +41,7 @@ Lemma falling_edge_compute_s_firable_true :
     γ ⊢ s ∼ σ ->
     
     (* Falling edge from s to s', s ⇝↓ s' *)
-    SitpnStateTransition Ec τ s s' falling_edge -> 
+    SitpnStateTransition Ec τ s s' fe -> 
 
     (* Falling edge from σ to σf *)
     vfalling Δ σ (get_behavior d) σ__f -> 
@@ -69,7 +69,7 @@ Lemma falling_edge_compute_s_firable_false :
     γ ⊢ s ∼ σ ->
     
     (* Falling edge from s to s', s ⇝↓ s' *)
-    SitpnStateTransition Ec τ s s' falling_edge -> 
+    SitpnStateTransition Ec τ s s' fe -> 
 
     (* Falling edge from σ to σf *)
     vfalling Δ σ (get_behavior d) σ__f -> 
@@ -97,7 +97,7 @@ Lemma falling_edge_compute_firable :
     γ ⊢ s ∼ σ ->
     
     (* Falling edge from s to s', s ⇝↓ s' *)
-    SitpnStateTransition Ec τ s s' falling_edge -> 
+    SitpnStateTransition Ec τ s s' fe -> 
 
     (* Falling edge from σ to σf *)
     vfalling Δ σ (get_behavior d) σ__f -> 
@@ -125,7 +125,7 @@ Lemma falling_edge_compute_nfirable :
     γ ⊢ s ∼ σ ->
     
     (* Falling edge from s to s', s ⇝↓ s' *)
-    SitpnStateTransition Ec τ s s' falling_edge -> 
+    SitpnStateTransition Ec τ s s' fe -> 
 
     (* Falling edge from σ to σf *)
     vfalling Δ σ (get_behavior d) σ__f -> 
@@ -290,7 +290,7 @@ Lemma elect_fired_compute_fired :
     γ ⊢ s ∼ σ ->
     
     (* Falling edge from s to s', s ⇝↓ s' *)
-    SitpnStateTransition Ec τ s s' falling_edge -> 
+    SitpnStateTransition Ec τ s s' fe -> 
 
     (* Falling edge from σ to σf *)
     vfalling Δ σ (get_behavior d) σ__f -> 
@@ -400,7 +400,7 @@ Lemma falling_edge_compute_fired_aux :
     γ ⊢ s ∼ σ ->
     
     (* Falling edge from s to s', s ⇝↓ s' *)
-    SitpnStateTransition Ec τ s s' falling_edge -> 
+    SitpnStateTransition Ec τ s s' fe -> 
 
     (* Falling edge from σ to σf *)
     vfalling Δ σ (get_behavior d) σ__f -> 
@@ -530,7 +530,7 @@ Lemma falling_edge_compute_fired_list :
     γ ⊢ s ∼ σ ->
     
     (* Falling edge from s to s', s ⇝↓ s' *)
-    SitpnStateTransition Ec τ s s' falling_edge -> 
+    SitpnStateTransition Ec τ s s' fe -> 
 
     (* Falling edge from σ to σf *)
     vfalling Δ σ (get_behavior d) σ__f -> 
@@ -625,7 +625,7 @@ Lemma elect_fired_compute_fired_port_false :
     γ ⊢ s ∼ σ ->
     
     (* Falling edge from s to s', s ⇝↓ s' *)
-    SitpnStateTransition Ec τ s s' falling_edge -> 
+    SitpnStateTransition Ec τ s s' fe -> 
 
     (* Falling edge from σ to σf *)
     vfalling Δ σ (get_behavior d) σ__f -> 
@@ -716,7 +716,7 @@ Lemma falling_edge_compute_fired_port_false_aux :
     γ ⊢ s ∼ σ ->
     
     (* Falling edge from s to s', s ⇝↓ s' *)
-    SitpnStateTransition Ec τ s s' falling_edge -> 
+    SitpnStateTransition Ec τ s s' fe -> 
 
     (* Falling edge from σ to σf *)
     vfalling Δ σ (get_behavior d) σ__f -> 
@@ -810,7 +810,7 @@ Lemma falling_edge_compute_fired_port_false_list :
     γ ⊢ s ∼ σ ->
     
     (* Falling edge from s to s', s ⇝↓ s' *)
-    SitpnStateTransition Ec τ s s' falling_edge -> 
+    SitpnStateTransition Ec τ s s' fe -> 
 
     (* Falling edge from σ to σf *)
     vfalling Δ σ (get_behavior d) σ__f -> 
@@ -1320,7 +1320,7 @@ Lemma elect_fired_compute_fired_port_true :
     γ ⊢ s ∼ σ ->
     
     (* Falling edge from s to s', s ⇝↓ s' *)
-    SitpnStateTransition Ec τ s s' falling_edge -> 
+    SitpnStateTransition Ec τ s s' fe -> 
 
     (* Falling edge from σ to σf *)
     vfalling Δ σ (get_behavior d) σ__f -> 
@@ -1433,7 +1433,7 @@ Lemma falling_edge_compute_fired_port_true_aux :
     γ ⊢ s ∼ σ ->
     
     (* Falling edge from s to s', s ⇝↓ s' *)
-    SitpnStateTransition Ec τ s s' falling_edge -> 
+    SitpnStateTransition Ec τ s s' fe -> 
 
     (* Falling edge from σ to σf *)
     vfalling Δ σ (get_behavior d) σ__f -> 
@@ -1524,7 +1524,7 @@ Lemma falling_edge_compute_fired_port_true_list :
     γ ⊢ s ∼ σ ->
     
     (* Falling edge from s to s', s ⇝↓ s' *)
-    SitpnStateTransition Ec τ s s' falling_edge -> 
+    SitpnStateTransition Ec τ s s' fe -> 
 
     (* Falling edge from σ to σf *)
     vfalling Δ σ (get_behavior d) σ__f -> 
@@ -1574,7 +1574,7 @@ Lemma falling_edge_compute_fired_port_true :
     γ ⊢ s ∼ σ ->
     
     (* Falling edge from s to s', s ⇝↓ s' *)
-    SitpnStateTransition Ec τ s s' falling_edge -> 
+    SitpnStateTransition Ec τ s s' fe -> 
 
     (* Falling edge from σ to σf *)
     vfalling Δ σ (get_behavior d) σ__f -> 
@@ -1621,7 +1621,7 @@ Lemma falling_edge_states_equal :
     γ ⊢ s ∼ σ ->
     
     (* Falling edge from s to s', s ⇝↓ s' *)
-    SitpnStateTransition Ec τ s s' falling_edge -> 
+    SitpnStateTransition Ec τ s s' fe -> 
 
     (* Falling edge from σ to σf *)
     vfalling Δ σ (get_behavior d) σ__f -> 
