soundness/InitialStates.v
@@ -1,0 +1,37 @@
+(** * Similar Initial States *)
+
+Require Import common.NatMap.
+
+Require Import sitpn.dp.SitpnSemantics.
+
+Require Import hvhdl.SemanticalDomains.
+Require Import hvhdl.DesignElaboration.
+Require Import hvhdl.AbstractSyntax.
+Require Import hvhdl.HilecopDesignStore.
+Require Import hvhdl.Initialization.
+
+Require Import sitpn2hvhdl.GenerateHVhdl.
+
+Require Import soundness.SoundnessDefs.
+
+(** ** Similar Initial States Lemma *)
+
+Lemma sim_init_states :
+  forall sitpn decpr id__ent id__arch mm d γ Δ σ__e σ0,
+    
+    (* [sitpn] translates into [(d, γ)]. *)
+    sitpn_to_hvhdl sitpn decpr id__ent id__arch mm = (inl (d, γ)) ->
+    
+    (* [Δ, σ__e] are the results of the elaboration of [d]. *)
+    edesign hdstore (empty value) d Δ σ__e ->
+
+    (* initialization d's state. *)
+    init Δ σ__e (behavior d) σ0 ->
+
+    (* init states are similar *)
+    γ ⊢ (s0 sitpn) ∼ σ0.
+Proof.
+  
+Admitted.
+
+Hint Resolve sim_init_states : core.
